\chapter{Equations and inequalities}

\begin{exercises}{}
{
Solve the following equations (assume all denominators are non-zero): \\
\begin{multicols}{2}
\begin{enumerate}[itemsep=6pt, label=\textbf{\arabic*}. ] 
\item   $2y-3=7$
\item   $-3y=0$        
\item   $16y+4=-10$        
\item   $12y+0=144$
\item   $7+5y=62$       
\item  $55=5x+\dfrac{3}{4}$ 
\item   $5x=2x+45$        
\item  $23x-12=6+3x$
\item   $12-6x+34x=2x-24-64$
\item   $6x+3x=4-5(2x-3)$
\item   $18-2p=p+9$   
\item   $\dfrac{4}{p}=\dfrac{16}{24}$
\item   $-(-16-p)=13p-1$
\item   $3f-10=10$
\item   $3f+16=4f-10$
\item   $10f+5=-2f-3f+80$
\item   $8(f-4)=5(f-4)$
\item  $6=6(f+7)+5f$      
\item $(a-1)^{2} - 2a = (a+3)(a-2) - 3$
\item $-7x = x+8(1-x)$ 
\item $5-\dfrac{7}{b} = \dfrac{2(b+4)}{b}$
\item $\dfrac{x+2}{4} - \dfrac{x-6}{3} = \dfrac{1}{2}$
\item $ 3 - \dfrac{y-2}{4} = 4$
\item $ \dfrac{a+1}{a+2} = \dfrac{a-3}{a+1}$
\end{enumerate}
\end{multicols}

}
\end{exercises}


 \begin{solutions}{}{
\begin{enumerate}[itemsep=5pt, label=\textbf{\arabic*}. ] 


\begin{enumerate}[itemsep=6pt, label=\textbf{\arabic*}. ] 
\item   $2y-3=7\\2y=10\\y=5$
\item   $-3y=0\\y=\frac{0}{3}\\y=0$        
\item   $16y+4=-10\\16y=-14\\y=-\frac{14}{16}\\=\frac{7}{8}$        
\item   $12y+0=144\\y=\frac{144}{12}\\y=12$
\item   $7+5y=62\\5y=62-7\\5y=11\\y=11$       
\item  $55=5x+\frac{3}{4}\\220=20x+3\\20x=117\\x=\frac{117}{20}$ 
\item   $5x=2x+45\\3x=45\\x=15$        
\item  $23x-12=6+3x\\20x=18\\x=\frac{18}{20}\\x=\frac{9}{10}$
\item   $12-6x+34x=2x-24-64\\-6x+34x-2x=-24-64-12\\ 26x=100\\x=\frac{100}{26}$
\item   $6x+3x=4-5(2x-3)\\6x+3x=4-10x+15\\19x=19\\x=1$
\item   $18-2p=p+9\\9=3p\\p=3$   
\item   $\frac{4}{p}=\frac{16}{24}\\96=16p\\p=6$
\item   $-(-16-p)=13p-1\\16+p=13p-1\\17=12p\\p=\frac{17}{12}$
\item   $3f-10=10\\3f=20\\f=\frac{20}{3}$
\item   $3f+16=4f-10\\-f=-10-16\\f=26$
\item   $10f+5=-2f-3f+80\\10f+2f+3f=75\\15f=75\\f=5$
\item   $8(f-4)=5(f-4)\\8f-32=5f-20\\3f=12\\f=4$
\item  $6=6(f+7)+5f\\6=6f+42+5f\\-36=11f\\f=-\frac{36}{11}$      
\item $(a-1)^{2} - 2a = (a+3)(a-2) - 3\\a^2-2a+1-2a=a^2-2a+3a-6-3\\-4a+1=a-9\\5a=10\\a=2$
\item $-7x = x+8(1-x)\\-7x=-7x+8\\0=8$\\ No solution 
\item $5-\dfrac{7}{b} = \dfrac{2(b+4)}{b}\\[4pt]5b-7=2(b+4)\\[4pt]5b-7=2b+8\\3b=15\\b=5$
\item $\dfrac{x+2}{4} - \dfrac{x-6}{3} = \dfrac{1}{2}\\[4pt]\dfrac{3(x=2)}{12}-\dfrac{4(x-6)}{12}=\frac{6}{12}\\[4pt]3(x+2)-4(x-6)=6\\[4pt]3x+6-4x+24=6\\-x=-24\\x=24$
\item $ 3 - \dfrac{y-2}{4} = 4\\[4pt]12-y-2=16\\-4=y+2\\y=-6$
\item $ \dfrac{a+1}{a+2} = \dfrac{a-3}{a+1}\\[4pt]\dfrac{a+1}{a+2} - \dfrac{a-3}{a+1}=0\\[4pt](a+1)^2 -(a-3)(a+2)=0\\a^2+2a+1-(a^2-a-6)=0\\a^2+2a+1-a^2+a+6=0\\3a+7=0\\a=-\frac{7}{3}$
\end{enumerate}

\end{enumerate}}
\end{solutions}



\begin{exercises}{ }
{
Solve the following equations:
\begin{multicols}{2}
\begin{enumerate}[itemsep=5pt, label=\textbf{\arabic*}. ] 
\item  $(3x+2)(3x-4)=0$
\item  $(5x-9)(x+6)=0$
\item  $(2y+3)(2y-3)=0$ 
\item  $(2x+1)(2x-9)=0$    
\item  $(4x)(x-3)=-9$       
\item  $20m+25{m}^{2}=0$
\item  $2{x}^{2}-5x-12=0$  
\item  $-75{x}^{2}+290x=240$
\item  $2x=\frac{1}{3}{x}^{2}-3x+14\frac{2}{3}$
\item  ${x}^{2}-4x=-4$      
\item  $-{x}^{2}+4x-6=4{x}^{2}-5x+3$       
\item  ${t}^{2}=3t$  
\item  ${x}^{2}-10x=-25$      
\item  ${x}^{2}=18$
\item  ${p}^{2}-6p=7$
\item  $4{x}^{2}-17x-77=0$
\item  $14{x}^{2}+5x=6$
\item  $2{x}^{2}-2x=12$              
\end{enumerate}
\end{multicols}

}
\end{exercises}


 \begin{solutions}{}{
\begin{enumerate}[itemsep=5pt, label=\textbf{\arabic*}. ] 


\item  $(3x + 2)(3x âˆ’ 4) = 0 \\ \therefore x=-\frac{2}{3}$ or $x=\frac{4}{3}$
\item $(5x-9)(x+6)=0\\ \therefore  x=\frac{9}{5}$ or $x=-6$% $$
\item $(2y+3)(2y-3)=0\\ \therefore  y=\frac{-3}{2}$ or $y=\frac{3}{2}$% $$ 
\item $x(2x+1)(2x-9)\\ \therefore x=-\frac{1}{2}$ or $x=\frac{9}{2}$% $=0$    
\item $(4x)(x-3)=-9\\4x^2-12x+9=0\\(2x-3)(2x-3)=0\\ \therefore x=\frac{3}{2}$% $$       
\item $20m+25{m}^{2}=0\\5m(4+5m)=0$\\ $\therefore  m=0$ or $m=\frac{-4}{5}$% $$
\item $2{x}^{2}-5x-12=0\\(2x+3)(x-4)=0\\ \therefore  x= 4$ or $\frac{-3}{2}$ % $$  
\item $-75{x}^{2}+290x=240\\-15x^2+58x-48=0\\(5x-6)(3x-8)\\ \therefore \x= frac{6}{5}$ or $x= \frac{8}{3}$% $$
\item $2x=\frac{1}{3}{x}^{2}-3x+14\frac{2}{3}\\2x=\frac{1}{3}x^2-3x+\frac{44}{3}\\6x=x^2-9x+44\\x^2-15x+44=0\\(x-4)(x-11)=0\\ \therefore   x=4$ or $x=11$% $$
\item ${x}^{2}-4x=-4\\(x-2)(x-2)=0\\ \therefore  x=2$% $$      
\item $-{x}^{2}+4x-6=4{x}^{2}-14x+3\\5x^2-18x+9=0\\(5x-3(x-3)=0\\ \therefore x=\frac{3}{5}$ or $x=3$% $$       
\item ${t}^{2}=3t\\t(t-3)=0\\ \therefore t=0$ or $t=3$% $$  
\item ${x}^{2}-10x=-25\\ x^2-10x+25=0\\(x-5)(x-5)=0\\ \therefore  x=5$% ${x}^{2}-10x=-25$      
\item ${x}^{2}=18\\ \therefore x=\sqrt{18}$ or $x=-\sqrt{18}$% $$
\item ${p}^{2}-6p=7\\ p^2-6p-7=0\\(p+1)(p-7)=0\\ \therefore p=-1$ or $p=7$% $$
\item $4{x}^{2}-17x-77=0\\(4x+11)(x-7)=0\\ \therefore x=7$ or $x=-\frac{11}{4}$% $$
\item $14{x}^{2}+5x=6\\14x^2 +5x-6=0\\(7x-3)(2x+2)=0\\ \therefore  x=\frac{3}{7}$ or $x=-\frac{1}{2}$% $$
\item $2{x}^{2}-2x=12\\ x^2-x-6=0\\(x-3)(x+2)=0\\ \therefore x=-2$ or $x=3$% $$   

\end{enumerate}}
\end{solutions}



\begin{exercises}{}
{
\Note{Solving a system of simultaneous equations graphically is sometimes not very accurate but provides a valuable method of solution.}
\begin{enumerate}[noitemsep, label=\textbf{\arabic*}. ] 
\item Solve algebraically: 
\begin{enumerate}[noitemsep, label=\textbf{(\alph*)} ] 
\item $3x-14y=0$ and $x-4y+1=0$
\item $x+y=8$ and $3x + 2y = 21$
\item $y=2x+1$ and $x + 2y + 3 = 0$
\end{enumerate}
\item Solve graphically and check your answer algebraically:
\begin{enumerate}[noitemsep, label=\textbf{(\alph*)} ] 
\item  $x+2y=1$ and $\frac{x}{3} + \frac{y}{2} = 1$
\item $5= x+y$ and $x = y-2$
\item $3x - 2y = 0$ and $x - 4y + 1 = 0$
\end{enumerate}
\end{enumerate}

}
\end{exercises}


 \begin{solutions}{}{
\begin{enumerate}[itemsep=10pt, label=\textbf{\arabic*}. ] 
\item Solve algebraically: 
\begin{enumerate}[noitemsep, label=\textbf{(\alph*)} ] 
\item $3x-14y=0\\\therefore 3x=14y\\ \therefore x=\frac{14}{3}y$\\ \\
 Substitute value of $x$ into second equation: \\
$x-4y+1=0\\ \therefore \frac{14}{3}y-14y+1=0\\ 14y-12y+3=0\\2y=-3\\y=-\frac{3}{2}$\\ \\
Substitute value of $y$ back into first equation:\\
$\therefore x=\frac{14 (-\frac{3}{2})}{3} = -7$\\
$y=-\frac{3}{2}$ and $x=-7$.

\item $x+y=8 \\ \therefore x=8-y$\\ \\
Substitute value of $x$ into second equation:\\
$3x+2y=21 \\ \therefore 3(8-y)+2y = 21\\ 24-3y+2y=21\\ -y=-3\\y=3\\ \\$
Substitute value of $y$ back into first equation:\\
$\therefore x=8-3=5$\\
$y=3$ and $x=5$

\item $y=2x+1 \\ \\$
Substitute value of $y$ into second equation:\\
$ x+2y+3=0\\ \therefore x+2(2x+1)+3=0\\ 
x+4x+2+3=0\\
5x=-5\\
\therefore x=-1$\\ \\
Substitute value of $x$ back into first equation:\\
$\therefore y=2(-1)+1=-1$\\
$y=-1$ and $x=-1$

\end{enumerate}
\item %Solve graphically and check your answer algebraically:
\begin{enumerate}[itemsep=20pt, label=\textbf{(\alph*)} ] 
\item  %$x+2y=1$ and $\frac{x}{3} + \frac{y}{2} = 1$\\
\\
\scalebox{0.9}{
\begin{pspicture}(-3,-2)(4,2)
% \psgrid[gridcolor=lightgray,gridlabels=0,gridwidth=0.5pt]
\psset{yunit=0.5,xunit=0.5}
\psaxes[dx=1,Dx=1,arrows=<->, labels=all](0,0)(-3,-5)(6,3)
\psplot[xunit=0.5,plotstyle=curve,arrows=<->]{-2}{10.5}{x 0.5 neg mul 0.5 add}
\psplot[xunit=0.5,plotstyle=curve,arrows=<->]{-1}{10.5}{x 0.67 neg mul 2 add}
\uput[l](4.5,1.5){$y=-\frac{2}{3}x+2$}
\uput[l](-0.8,0.8){$y=-\frac{1}{2}x+\frac{1}{2}$}
% \uput[l](0.1,-0.2){$0$}
\uput[r](6,0.1){$x$}
\uput[r](0,3){$y$}
\psdot(4.5,-4)
\psline[linestyle=dotted](4.5,-4)(4.5,0)
\psline[linestyle=dotted](0,-4)(4.5,-4)
% \psline[arrows=<->](-4,1)(4,1)
\end{pspicture}
}\\
$x+2y=1$\\ $\therefore x=-2y+1\\$ \\ Substitute value of $x$ into the second equation:\\$\therefore \frac{-2y+1}{3} +\frac{y}{2} = 1\\
2(-2y+1) +3y=6\\
-4y+2+3y=6\\
\therefore y=-4$\\ \\
Substitute value of $y$ back into the first equation:\\
$x+2(-4)=1\\
x-8=1\\
\therefore x=9$


\item %$5= x+y$ and $x = y-2$\\
\\
\scalebox{0.9}{
\begin{pspicture}(-3,-2)(4,2)
% \psgrid[gridcolor=lightgray,gridlabels=0,gridwidth=0.5pt]
\psset{yunit=0.5,xunit=0.5}
\psaxes[dx=1,Dx=1,dy=1, Dy=1,arrows=<->](0,0)(-3,-5)(8,6)
\psplot[xunit=1,plotstyle=curve,arrows=<->]{-1}{6}{x 1 neg mul 5 add}
\psplot[xunit=1,plotstyle=curve,arrows=<->]{-1}{6}{x 2 sub}
\uput[l](4.5,4.4){$y=-x+5$}
\uput[l](3.8, -1.5){$y=x-2$}
\uput[l](0.1,-0.4){$0$}
\uput[r](8,0.1){$x$}
\uput[r](0,6){$y$}
\psdot(3.5,1.5)
\psline[linestyle=dotted](3.5,1.5)(3.5,0)
\psline[linestyle=dotted](0,1.5)(3.5,1.5)
% \psline[arrows=<->](-4,1)(4,1)
\end{pspicture}}\\
$5=x+y\\ 
\therefore y=5-x$\\ \\
Substitute value of $y$ into second equation:\\
$x=5-x-2$\\
$2x=3\\
\therefore x=\frac{3}{2}$\\ \\
Substitute value of $x$ back into first equation:\\
$5=\frac{3}{2} +y\\
y=\frac{10}{2} - \frac{3}{2} = \frac{7}{2}$

\item %$3x - 2y = 0$ and $x - 4y + 1 = 0$\\
\\
\scalebox{1}{
\begin{pspicture}(-3,-2)(4,2)
% \psgrid[gridcolor=lightgray,gridlabels=0,gridwidth=0.5pt]
\psset{yunit=0.5,xunit=0.5}
\psaxes[dx=1,Dx=1,dy=1, Dy=1,arrows=<->](0,0)(-3,-5)(4,5)
\psplot[xunit=1,plotstyle=curve,arrows=<->]{-1.5}{3}{x 1.5 mul}
\psplot[xunit=1,plotstyle=curve,arrows=<->]{-2}{4}{x 0.25 mul 0.25 add}
\uput[l](4.5,4.7){$y=\frac{3}{2}x$}
\uput[ul](5.4, 1){$y=\frac{1}{4}x+\frac{1}{4}$}
\uput[l](0.1,-0.4){$0$}
\uput[r](4,0.1){$x$}
\uput[r](0,5){$y$}
\psdot(0.2,0.3)
\psline[linestyle=dotted,dotsep=0.01](0.2,0.3)(0.2,0)
\psline[linestyle=dotted](0,0.3)(0.2,0.3)
% \psline[arrows=<->](-4,1)(4,1)
\end{pspicture}}\\
$3x-2y=0\\
\therefore y=\frac{3}{2}x$\\ \\
Substitute value of $y$ into second equation:\\
$\therefore x-4\left(\frac{3}{2}x\right) +1 = 0\\
x-6x+1 = 0\\
5x=1\\
x=\frac{1}{5}\\$ \\
Substitute value of $x$ back into first equation:\\
$3\frac{1}{5} - 2y=0\\
3-10y=0\\
10y=3\\
y=\frac{3}{10}$
\end{enumerate}
\end{enumerate}}
\end{solutions}



\begin{exercises}{}
{
\begin{enumerate}[noitemsep, label=\textbf{\arabic*}. ] 
\item Two jets are flying towards each other from airports that are $1~200$ km apart. One jet is flying at $250$ km/h and the other jet at $350$ km/h. If they took off at the same time, how long will it take for the jets to pass each other?
\item Kadesh bought $20$ shirts at a total cost of R$~980$. If the
  large shirts cost R$~50$ and the small shirts cost R$~40$. How many
  of each size did he buy?
\item The diagonal of a rectangle is $25~$cm more than its width. The length of the rectangle is $17~$cm more than its width. What are the dimensions of the rectangle?  
\item The sum of $27$ and $12$ is equal to $73$ more than an unknown number. Find the unknown number.
\item The two smaller angles in a right-angled triangle are in the ratio of $1:2$. What are the sizes of the two angles? 
\item The length of a rectangle is twice the breadth. If the area is $128$ cm$^{2}$, determine the length and the breadth.       
\item If $4$ times a number is increased by $7$, the result is $15$ less than the square of the number. Find the number.
\item The length of a rectangle is $2~$cm more than the width of the rectangle. The perimeter of the rectangle is $20~$cm. Find the length and the width of the rectangle.
\item Stephen has $1~\ell{}$ of a mixture containing $69\%$ salt. How much water must Stephen add to make the mixture $50\%$ salt? Write your answer as a fraction of a litre.
\end{enumerate}

}
\end{exercises}


 \begin{solutions}{}{
\begin{enumerate}[itemsep=10pt, label=\textbf{\arabic*}. ] 


\item Let distance $d_1=1~200-x$ km and $d_2=x$ km; \\
speed $S_1=250$ km/h and $S_2=350$ km/h. \\
$\mbox{Time } t = \dfrac{\mbox{Distance}}{\mbox{Speed}} \\[5pt]$
When the jets pass each other $\dfrac{1~200-x}{250} = \dfrac{x}{350}\\[5pt]
350(1~200-x)=250x\\
420~000 - 350x = 250x\\
600x = 420~000\\
x= 700$ km\\[5pt]

$\therefore t=\dfrac{700\mbox{ km}}{350{\mbox{ km/h}}}\\[5pt]
=2$ hours\\
It will take take the jets $2$ hours to pass each other.

\item\\
Populate the data in a table format (let $x=$ the number of large shirts):\\
  \begin{tabularx}{8cm}{ |X|X|X|X| }\hline
& Nr shirts & Cost & Total \\ \hline
Large & $x$ & $50$ & $980$\\ \hline
Small & $20-x$ & $40$&\\ \hline
\end{tabularx}\\
\\
$50x+40(20-x)=980\\
50x+800-40x=980\\
10x=180\\
\therefore x=18\\$
Kadesh buys $18$ large shirts and $2$ small shirts.

\item Let length $=l$, width $=w$ and diagonal $=d$.\\
$\therefore d=w+25$ and $l=w+17$.\\
By the theorem of Pythagoras:\\
$d^2 = l^2+w^2\\
\therefore w^2 = d^2-l^2\\
=(w+25)^2 - (w+17)^2\\
=w^2+50w+625-w^2-34w-289\\
\therefore w^2 - 16w - 336 = 0\\
(w+12)(w-28)=0\\
\therefore w= -12$ or $w=28$\\
The width must be positive, therefore \\
$w=28$ cm\\ 
$l=(w+17)=45$ cm \\
and $d=(w+25)=53$ cm.


\item Let the unkown number $=x$\\
$\therefore 27+12=x+73\\
39=x+73\\
x=39-73\\
x=-34\\$

\item Let $x=$ the smallest angle. Therefore the other angle $=2x$. \\
We are given the third angle $=90^{\circ}$. \\
$x+2x+90^{\circ} = 180^{\circ}$ (sum of angles in a triangle)\\
$\therefore 3x = 90^{\circ}\\
\therefore x= 30^{\circ}$\\
The sizes of the angles are $30^{\circ}$ and $60^{\circ}$. 
\item 
We are given length $l=2b$ and $l\times b=128$\\
$\therefore 2b\times b =128\\
2b^2=128\\
b^2=64\\
b=\pm8\\$
But breadth must be positive, therefore $b=8$ cm, and $l=2b=16$ cm.
\item Let the number $=x$. \\
Therefore the equation is $4x+6=x^2-15$.\\
$\therefore x^2-4x-21=0\\
(x-7)(x+3)=0\\
x=7$ or $x=-3$
\item Let length $l=x$, width $w=x-2$ and perimeter $=p$\\
$\therefore p = 2l+2w\\
=2x+2(x-2)\\
20=2x+2x-4\\
4x=24\\
x=6$\\
$\therefore$ $l=6$ cm and $w=l-2=4$ cm.
\item solution 9

\end{enumerate}}
\end{solutions}



\begin{exercises}{}
{
\begin{enumerate}[itemsep=5pt, label=\textbf{\arabic*}. ] 
\item Solve for $a$: $s=ut+\frac{1}{2}at^{2}$
\item Solve for $n$: $pV=nRT$ 
\item Solve for $x$: $\dfrac{1}{b}+\dfrac{2b}{x}=2$
\item Solve for $r$: $V = \pi r^{2} h$
\item Solve for $h$: $E=\dfrac{hc}{\lambda}$
\item Solve for $h$: $A=2\pi rh + 2 \pi r$
\item Solve for $\lambda$: $t=\dfrac{D}{f \lambda}$
\item Solve for $m$: $E=mgh + \frac{1}{2}mv^{2}$
\end{enumerate}

}
\end{exercises}


 \begin{solutions}{}{
\begin{enumerate}[itemsep=5pt, label=\textbf{\arabic*}. ] 


\item solution 1
\item solution 2
\item solution 3
\item solution 4
\item solution 5
\item solution 6
\item solution 7
\item solution 8

\end{enumerate}}
\end{solutions}



\begin{exercises}{ }
{
Solve for $x$ and represent the answer on a number line and in interval notation:
\begin{enumerate}[itemsep=6pt, label=\textbf{\arabic*}. ] 
    \item $3x+4>5x+8$
    \item $3(x-1)-2\leq 6x+4$ 
    \item $\dfrac{x-7}{3}>\dfrac{2x-3}{2}$
    \item $-4(x-1)<x+2$
    \item $\dfrac{1}{2}x+\dfrac{1}{3}(x-1)\geq \dfrac{5}{6}x-\dfrac{1}{3}$ 
    \item $-2\leq x-1<3$ 
    \item $-5<2x-3\leq7$ 
\item $7(3x+2)-5(2x-3)>7$
    \end{enumerate}

}
\end{exercises}


 \begin{solutions}{}{
\begin{enumerate}[itemsep=5pt, label=\textbf{\arabic*}. ] 


\item solution 1
\item solution 2
\item solution 3
\item solution 4
\item solution 5
\item solution 6
\item solution 7
\item solution 8

\end{enumerate}}
\end{solutions}


\begin{eocexercises}{}
\begin{enumerate}[itemsep=5pt, label=\textbf{\arabic*}. ] 
 \item 
Solve:
\begin{enumerate}[itemsep=6pt,label=\textbf{(\alph*)}]
\begin{multicols}{2} 
\item $2(p-1) = 3(p+2)$
\item $3-6k = 2k-1$
\item $m + 6(-m+1) + 5m = 0$
\item $2k + 3 = 2-3(k+3)$
\item $5t-1=t^{2}-(t+2)(t-2)$\
\item $3+\dfrac{q}{5} = \dfrac{q}{2}$ 
\item $5-\dfrac{2(m+4)}{m} = \dfrac{7}{m}$
\item $\dfrac{2}{t} - 2 - \dfrac{1}{2} = \dfrac{1}{2}\left(1+\dfrac{2}{t}\right)$
\item $x^{2} - 3x + 2=0$
\item $y^{2} + y = 6$
\item $0=2x^{2} - 5x - 18$
\item $(d+4)(d-3)-d=(3d-2)^{2} - 8d(d-1)$
\item $5x+2\leq4(2x-1)$
\item $\dfrac{4x-2}{6} > 2x+1$
\item $\dfrac{x}{3} - 14 > 14 - \dfrac{x}{7}$
\item $\dfrac{1-a}{2} - \dfrac{2-a}{3} \geq 1$
\item $-5 \leq 2k + 1 < 5$
\item $x-1=\dfrac{42}{x}$  
\end{multicols}
\end{enumerate}
\item Consider the following literal equations:
\begin{enumerate}[itemsep=6pt,label=\textbf{(\alph*)}]
\item Solve for $I$: $P = VI$
\item Solve for $m$: $E=mc^{2}$
\item Solve for $t$: $v = u + at$
\item Solve for $f$: $\dfrac{1}{u} + \dfrac{1}{v} = \dfrac{1}{f}$
\item Solve for $C$: $F=\frac{9}{5}C + 32$
\item Solve for $y$: $m = \dfrac{y-c}{x}$
\end{enumerate}
\item Solve the following simultaneous equations:
\begin{enumerate}[itemsep=5pt,label=\textbf{(\alph*)}]
\item $7x+3y=13$ and $2x-3y=-4$  
\item $10=2x+y$ and $y=x-2$
\item $7x-41=3y$ and $17=3x-y$
\item $2y=x+8$ and $4y=2x-44$
\end{enumerate}
\item Find the solutions to the following word problems:
\begin{enumerate}[itemsep=5pt,label=\textbf{(\alph*)}]
\item $\frac{7}{8}$ of a certain number is $5$ more than of $\frac{1}{3}$ of the number. Find the number.
\item Three rulers and two pens have a total cost of R $21,00$. One ruler and one pen have a total cost of R $8,00$. How much does a ruler cost and how much does a pen cost? 
\item A man runs to the bus stop and back in $15$ minutes. His speed on the way to the bus stop is $5$ km/h and his speed on the way back is $4$ km/h. Find the distance to the bus stop.
\item Zanele and Piet skate towards each other on a straight path. They set off $20$ km apart. Zanele skates at $15$ km/h and Piet at $10$ km/h. How far will Piet have skated when they reach each other?
\item When the price of chocolates is increased by R $10$, we can buy five fewer chocolates for R $300$. What was the price of each chocolate before the price was increased?
\end{enumerate}
\end{enumerate}

\end{eocexercises}


 \begin{solutions}{}{
\begin{enumerate}[itemsep=5pt, label=\textbf{\arabic*}. ] 


\item solution 1
\item solution 2
\item solution 3
\item solution 4

\end{enumerate}}
\end{solutions}


